veric/external_state.v
@@ -1,0 +1,22 @@
+From iris.algebra Require Export excl.
+From iris_ora.algebra Require Export excl.
+From iris_ora.logic Require Export own.
+From VST.veric Require Export base dfrac auth res_predicates.
+
+(* external ghost state *)
+Lemma excl_orderN_includedN : forall {A : ofe} n (x y : excl' A), x ≼ₒ{n} y → x ≼{n} y.
+Proof.
+  intros.
+  destruct x, y; simpl in *; try done.
+  - exists None; rewrite right_id; constructor; done.
+  - eexists; rewrite left_id //.
+Qed.
+
+Canonical Structure excl_authR (A : ofe) := authR (optionUR (@exclR A)) excl_orderN_includedN.
+
+Class externalGS (Z : Type) (Σ : gFunctors) := ExternalGS {
+  external_inG : inG Σ (excl_authR (leibnizO Z));
+  external_name : gname
+}.
+
+Definition has_ext `{heapGS Σ} `{!externalGS Z Σ} (z : Z) : mpred := own(inG0 := external_inG) external_name (◯ Excl' z).
